theories/step.v
@@ -1,4 +1,5 @@
-Require Import lang base free eval.
+From stdpp Require Import gmap.
+Require Import lang base free eval store.
 
 (* This file defines an ample-step semantics, that is, a reduction semantics
    of the form [step m m'] where [m] and [m'] are computations in the [free]
@@ -10,6 +11,12 @@ Require Import lang base free eval.
 (* Working directly with the relation [step] removes the need to transport
    computations from the free monad into some other monad. (This was the
    job of the function [handle] defined in handle.v.) *)
+
+(* -------------------------------------------------------------------------- *)
+(* The state of an execution is a term of type [free A] taken together with
+   a store. *)
+Definition state (A : Type) : Type := store * free A.
+
 
 (* -------------------------------------------------------------------------- *)
 
@@ -24,83 +31,114 @@ Require Import lang base free eval.
    is [Fail]. There is a lot of non-determinism in these reduction rules:
    e.g., [Par Fail Next _ _] can reduce to either [Fail] or [Next]. *)
 
-Inductive step {A} : free A → free A → Prop :=
+Inductive step {A} : state A → state A → Prop :=
 
   (* [Stop Eval (η, e) k] steps to an invocation of [eval η e] followed
      with the continuation [k]. *)
   (* Isolating an explicit equality [p = (η, e)] seems necessary to work
      around a bug or limitation (?) in [dependent destruction]. *)
   | StepEval :
-      ∀ p η e k,
+      ∀ σ p η e k,
       p = (η, e) →
       step
-        (Stop Eval p k)
-        (bind (eval η e) k)
+        (σ, Stop Eval p k)
+        (σ, bind (eval η e) k)
 
   (* [Stop Loop (η, x, i1, i2, e) k] steps to [loop η x i1 i2 e] followed
      with the continuation [k]. *)
   | StepLoop :
-      ∀ p η x i1 i2 e k,
+      ∀ σ p η x i1 i2 e k,
       p = (η, x, i1, i2, e) →
       step
-        (Stop Loop p k)
-        (bind (loop η x i1 i2 e) k)
+        (σ, Stop Loop p k)
+        (σ, bind (loop η x i1 i2 e) k)
 
   (* [Stop Flip () k] steps to an application of the continuation [k] to
      either [false] or [true]. *)
   | StepFlip :
-      ∀ b x k,
+      ∀ σ b x k,
       step
-        (Stop Flip x k)
-        (k b)
+        (σ, Stop Flip x k)
+        (σ, k b)
+
+  (* [Stop Ref v] adds a fresh location in the store and stores [v] there; and
+      steps to an application of the continuation [k] to this location. *)
+  | StepStopRef :
+      ∀ σ v k,
+      let '(l, σ') := store_ref σ v in
+      step
+        (σ, Stop Ref v k)
+        (σ', k l)
+
+  | StepStopLoadSuccess :
+      ∀ σ l k (H: l ∈ dom σ),
+      let v := store_load σ l H in
+      step
+        (σ, Stop Load l k)
+        (σ, k v)
+
+  | StepStopLoadFailure :
+      ∀ σ l k (H: l ∉ dom σ),
+      step
+        (σ, Stop Load l k)
+        (σ, Fail)
+
+  | StepStopStoreSuccess :
+      ∀ σ l v k (H: l ∈ dom σ),
+      step (σ, Stop Store (l, v) k) (<[ l := v]> σ, k tt)
+
+  | StepStopStoreFailure :
+      ∀ σ (l: loc) v k (H: l ∉ dom σ),
+      step
+        (σ, Stop Store (l, v) k)
+        (<[ l := v ]>σ, Fail)
 
   (* If [m1] and [m2] have reached values [v1] and [v2],
      then the continuation [k] is applied to the pair [(v1, v2)]. *)
   | StepParRetRet :
-      ∀ {A1 A2} (v1 : A1) (v2 : A2) k ko,
+      ∀ {A1 A2} σ (v1 : A1) (v2 : A2) k ko,
       step
-        (Par (Ret v1) (Ret v2) k ko)
-        (k (v1, v2))
+        (σ, Par (Ret v1) (Ret v2) k ko)
+        (σ, k (v1, v2))
 
   (* A hard failure on either side can be propagated up. *)
   | StepParFailLeft :
-      ∀ {A1 A2} m2 (k : A1 * A2 → free A) ko,
+      ∀ {A1 A2} σ m2 (k : A1 * A2 → free A) ko,
       step
-        (Par Fail m2 k ko)
-        Fail
+        (σ, Par Fail m2 k ko)
+        (σ, Fail)
   | StepParFailRight :
-      ∀ {A1 A2} m1 (k : A1 * A2 → free A) ko,
+      ∀ {A1 A2} σ m1 (k : A1 * A2 → free A) ko,
       step
-        (Par m1 Fail k ko)
-        Fail
+        (σ, Par m1 Fail k ko)
+        (σ, Fail)
 
   (* If a soft failure on either side is detected, then
      the failure continuation [n] can be invoked. *)
   | StepParNextLeft :
-      ∀ {A1 A2} m2(k : A1 * A2 → free A) ko,
+      ∀ {A1 A2} σ m2(k : A1 * A2 → free A) ko,
       step
-        (Par Next m2 k ko)
-        (ko())
+        (σ, Par Next m2 k ko)
+        (σ, ko())
   | StepParNextRight :
-      ∀ {A1 A2} m1 (k : A1 * A2 → free A) ko,
+      ∀ {A1 A2} σ m1 (k : A1 * A2 → free A) ko,
       step
-        (Par m1 Next k ko)
-        (ko())
+        (σ, Par m1 Next k ko)
+        (σ, ko())
 
   (* Reduction steps on either side are permitted. *)
   | StepParLeft :
-      ∀ {A1 A2} (m1 m'1 : free A1) (m2 : free A2) k ko,
-      step m1 m'1 →
+      ∀ {A1 A2} σ σ' (m1 m'1 : free A1) (m2 : free A2) k ko,
+      step (σ, m1) (σ', m'1) →
       step
-        (Par m1 m2 k ko)
-        (Par m'1 m2 k ko)
+        (σ, Par m1 m2 k ko)
+        (σ', Par m'1 m2 k ko)
   | StepParRight :
-      ∀ {A1 A2} (m1 : free A1) {m2 m'2 : free A2} k ko,
-      step m2 m'2 →
+      ∀ {A1 A2} σ σ' (m1 : free A1) {m2 m'2 : free A2} k ko,
+      step (σ, m2) (σ', m'2) →
       step
-        (Par m1 m2 k ko)
-        (Par m1 m'2 k ko)
-
+        (σ, Par m1 m2 k ko)
+        (σ', Par m1 m'2 k ko)
 .
 
 Global Hint Constructors step : step.
@@ -144,8 +182,8 @@ Ltac destruct_answer :=
 
 (* [m] can step if there exists [m'] such that [m] steps to [m']. *)
 
-Definition can_step {A} (m : free A) :=
-  ∃ m', step m m'.
+Definition can_step {A} (s : state A) :=
+  ∃ s', step s s'.
 
 Global Hint Unfold can_step : step.
 
@@ -153,9 +191,11 @@ Global Hint Unfold can_step : step.
 
 (* A term that is not an answer and that is unable to step is stuck. *)
 
-Definition stuck {A} (m : free A) :=
-  ¬ is_answer m ∧
-  (∀ m', ¬ step m m').
+Definition stuck {A} (m : state A) :=
+  match m with
+  | (σ, m) => ¬ is_answer m ∧
+             (∀ m' σ', ¬ step (σ, m) (σ', m'))
+  end.
 
 (* -------------------------------------------------------------------------- *)
 
@@ -164,21 +204,46 @@ Definition stuck {A} (m : free A) :=
 (* This auxiliary lemma is useful when a constructor of the relation [step]
    cannot be applied directly. *)
 
-Lemma step_eq {A} (m1 m2 m2' : free A) :
-  step m1 m2 →
-  m2 = m2' →
-  step m1 m2'.
+Lemma step_eq {A} (s1 s2 s2' : state A) :
+  step s1 s2 →
+  s2 = s2' →
+  step s1 s2'.
 Proof.
   intros. subst. assumption.
 Qed.
 
 (* [Stop] can step. *)
 
-Lemma can_step_stop {A X Y} (c : code X Y) x (k : Y → free A) :
-  can_step (Stop c x k).
+Lemma can_step_stop {A X Y} (σ: store) (c : code X Y) x (k : Y → free A) :
+  can_step (σ, Stop c x k).
 Proof.
-  unfold can_step. destruct c; repeat destruct x as (x & ?);
-  eauto using (StepFlip false), StepEval, StepLoop.
+  eauto with step.
+  destruct c; repeat destruct x as (x & ?).
+  - exists (σ, bind (eval x e) k). apply StepEval, eq_refl.
+  - exists (σ, bind (loop x v i0 i e) k). apply StepLoop, eq_refl.
+  - exists (σ, k false). apply StepFlip.
+  - set ℓ := fresh_locs (dom σ).
+    exists (<[ℓ:=x]> σ, k ℓ). apply StepStopRef.
+  - (* TODO: destruct the "belongs to" predicate instead of the result of
+     *       lookup. *)
+    destruct (σ !! x) eqn:E.
+    + (* The load operation will succeed. *)
+      apply elem_of_dom_2 in E.
+      exists (σ, k (store_load σ x E)).
+      apply StepStopLoadSuccess.
+    + (* The load operation will fail. *)
+      exists (σ, Fail). apply StepStopLoadFailure.
+      apply not_elem_of_dom_2, E.
+  - (* TODO: ditto. *)
+    destruct (σ !! x) eqn:E.
+    + (* The store operation will succeed. *)
+      apply elem_of_dom_2 in E.
+      exists (store_store σ x v E, k tt).
+      by apply StepStopStoreSuccess.
+    + (* The store operation will fail. *)
+      apply not_elem_of_dom_2 in E.
+      exists (<[ x := v ]> σ, Fail).
+      by apply StepStopStoreFailure.
 Qed.
 
 Global Hint Resolve can_step_stop : step.
@@ -186,23 +251,25 @@ Global Hint Resolve can_step_stop : step.
 (* The following auxiliary lemma is used in the proof of [can_step_par],
    which establishes a stronger result. *)
 
-Local Lemma can_step_under_par {A1 A2 A} m1 m2 (k : A1 * A2 → free A) ko :
-  can_step m1 ∨ can_step m2 →
-  can_step (Par m1 m2 k ko).
+Local Lemma can_step_under_par {A1 A2 A} σ m1 m2 (k : A1 * A2 → free A) ko :
+  can_step (σ, m1) ∨ can_step (σ, m2) →
+  can_step (σ, Par m1 m2 k ko).
 Proof.
-  unfold can_step.
-  intros [ (m'1 & ?) | (m'2 & ?) ]; eauto with step.
+  unfold can_step. eauto with step.
+  intros[[[]]|[[]]]. (* TODO: restore the previous proof relying on [eauto]. *)
+  - eexists _. apply StepParLeft, H.
+  - eexists _. apply StepParRight, H.
 Qed.
 
 (* [Par] can step. *)
 
 Lemma can_step_par :
-  ∀ {A} (m : free A) {A1 A2} m1 m2 (k : A1 * A2 → free A) ko,
+  ∀ {A} (m : free A) {A1 A2} σ m1 m2 (k : A1 * A2 → free A) ko,
   m = Par m1 m2 k ko →
-  can_step m.
+  can_step (σ, m).
 Proof.
   induction m; try solve [ congruence ].
-  intros A'1 A'2 m'1 m'2 k' ko' Heq.
+  intros A'1 A'2 σ' m'1 m'2 k' ko' Heq.
   (* The hypothesis [Heq] is tricky because it involves different types
      on either side. Fortunately, [dependent destruction] is capable
      of deconstructing it for us. Phew! *)
@@ -217,13 +284,17 @@ Global Hint Resolve can_step_par : step.
 
 (* This corresponds to reduction under an evaluation context. *)
 
-Lemma step_bind {A B} (m m' : free A) (f : A → free B) :
-  step m m' →
-  step (bind m f) (bind m' f).
+Lemma step_bind {A B} (σ σ': store) (m m' : free A) (f : A → free B) :
+  step (σ, m) (σ', m') →
+  step (σ, (bind m) f) (σ', (bind m') f).
 Proof.
   inversion 1; subst;
-  rewrite ?bind_stop, ?bind_par, ?bind_fail, ?bind_bind;
-  eauto using step_eq with step.
+  rewrite ?bind_stop ?bind_par ?bind_fail ?bind_bind;
+  eauto using step_eq with step;
+  eauto using StepFlip, step_eq with step.
+  (* TODO: improve the way the new cases are handeled. *)
+  - by pose proof (StepStopRef σ v (λ v0 : loc, bind (k v0) f)) as Hstep.
+  - by pose proof (StepStopLoadSuccess σ' l (λ v1 : val, bind (k v1) f) H3) as Hstep.
 Qed.
 
 (* Conversely, if [bind m f] takes a step, then this must be either because
@@ -234,13 +305,13 @@ Qed.
 
 Local Hint Extern 1 (_ = _) => rewrite bind_bind : bind_bind.
 
-Lemma invert_step_bind {A B} (m : free A) (f : A → free B) (b' : free B) :
-  step (bind m f) b' →
-  (∃ m', step m m' ∧ b' = bind m' f) ∨
-  (∃ a, m = Ret a ∧ step (f a) b').
+Lemma invert_step_bind {A B} σ (m : free A) (f : A → free B) (b' : state B) :
+  step (σ, bind m f) b' →
+  (∃ m' σ', step (σ, m) (σ', m') ∧ b' = (σ', bind m' f)) ∨
+  (∃ a, m = Ret a ∧ step (σ, f a) b').
 Proof.
   destruct m;
-  rewrite ?bind_ret, ?bind_stop, ?bind_par, ?bind_fail;
+  rewrite ?bind_ret ?bind_stop ?bind_par ?bind_fail;
   intro;
   try solve [
     (* Case: [Ret] *)
@@ -248,6 +319,18 @@ Proof.
   | (* Every other case: *)
     left; destruct_step; eauto with step bind_bind
   ].
+  (* TODO: unify the Stop case with the others. *)
+  left; destruct_step; unshelve eauto with step bind_bind.
+  - pose proof (StepEval σ (η, e) η e k (eq_refl (η, e))) as Hstep.
+    exists (bind (eval η e) k), σ.
+    split; eauto with step bind_bind.
+  - pose proof (StepLoop σ (η, x0, i1, i2, e) η x0 i1 i2 e k (eq_refl _)).
+    exists (bind (loop η x0 i1 i2 e) k), σ.
+    split; eauto with step bind_bind.
+  - pose proof (StepStopRef σ x k).
+    simpl in H.
+    exists (k (fresh_locs (dom σ))), (<[fresh_locs (dom σ):=x]> σ).
+    split; eauto with step bind_bind.
 Qed.
 
 (* -------------------------------------------------------------------------- *)
@@ -267,8 +350,8 @@ Qed.
 
 (* [Ret a] cannot step. *)
 
-Lemma invert_can_step_Ret {A} (a : A) :
-  can_step (Ret a) →
+Lemma invert_can_step_Ret {A} σ (a : A) :
+  can_step (σ, Ret a) →
   False.
 Proof.
   intros (m' & ?). destruct_step.
@@ -276,8 +359,8 @@ Qed.
 
 (* [Fail] cannot step. *)
 
-Lemma invert_can_step_Fail {A} :
-  can_step (Fail : free A) →
+Lemma invert_can_step_Fail {A} σ :
+  can_step (σ, Fail : free A) →
   False.
 Proof.
   intros (m' & ?). destruct_step.
@@ -285,8 +368,8 @@ Qed.
 
 (* [Next] cannot step. *)
 
-Lemma invert_can_step_Next {A} :
-  can_step (Next : free A) →
+Lemma invert_can_step_Next {A} σ :
+  can_step (σ, Next : free A) →
   False.
 Proof.
   intros (m' & ?). destruct_step.
@@ -300,17 +383,17 @@ Global Hint Resolve
 
 (* Stepping in the left-hand side of [bind] is permitted. *)
 
-Lemma can_step_bind {A B} (m : free A) (f : A → free B) :
-  can_step m →
-  can_step (bind m f).
+Lemma can_step_bind {A B} σ (m : free A) (f : A → free B) :
+  can_step (σ, m) →
+  can_step (σ, bind m f).
 Proof.
-  unfold can_step. intros (m' & Hstep). eauto using step_bind.
+  unfold can_step. intros ([] & Hstep). eauto using step_bind.
 Qed.
 
 (* A term that can step is not an answer. *)
 
-Lemma can_step_not_answer {A} (m : free A) :
-  can_step m →
+Lemma can_step_not_answer {A} σ (m : free A) :
+  can_step (σ, m) →
   ¬ is_answer m.
 Proof.
   intros.
@@ -322,16 +405,15 @@ Qed.
    a step (under a context). In other words, reduction under a context is
    mandatory: no other reduction is possible. *)
 
-Lemma invert_step_bind' {A B} (m : free A) (f : A → free B) (b' : free B) :
-  step (bind m f) b' →
+Lemma invert_step_bind' {A B} σ (m : free A) (f : A → free B) (b' : state B) :
+  step (σ, bind m f) b' →
   ¬ is_answer m →
-  (∃ m', step m m' ∧ b' = bind m' f).
+  (∃ σ' m', step (σ, m) (σ', m') ∧ b' = (σ', bind m' f)).
 Proof.
   intros Hstep Hnoret.
-  specialize (invert_step_bind _ _ _ Hstep).
-  intros [ ? | (a & ? & ?) ].
+  pose proof (invert_step_bind σ m f b' Hstep) as [(?&?&Hstep'&->)|(?&->&?)].
   { eauto. }
-  { subst m. false. simpl in Hnoret. tauto. }
+  { exfalso. by apply Hnoret. }
 Qed.
 
 (* -------------------------------------------------------------------------- *)
@@ -340,9 +422,9 @@ Qed.
 
 (* An answer is not stuck. *)
 
-Lemma invert_stuck_answer {A} (m : free A) :
+Lemma invert_stuck_answer {A} (m : free A) σ :
   is_answer m →
-  stuck m →
+  stuck (σ, m) →
   False.
 Proof.
   unfold stuck. tauto.
@@ -350,29 +432,29 @@ Qed.
 
 (* A term that can step is not stuck. *)
 
-Lemma can_step_not_stuck {A} (m : free A) :
-  can_step m →
-  stuck m →
+Lemma can_step_not_stuck {A} (m : free A) σ :
+  can_step (σ, m) →
+  stuck (σ, m) →
   False.
 Proof.
   unfold can_step, stuck.
-  intros (m' & Hstep).
+  intros ([] & Hstep).
   intros (_ & Hnostep).
   eapply Hnostep. exact Hstep.
 Qed.
 
 (* [Fail] is stuck. *)
 
-Lemma stuck_Fail {A} :
-  stuck (Fail : free A).
+Lemma stuck_Fail {A} σ :
+  stuck (σ, Fail : free A).
 Proof.
   unfold stuck. split. eauto. inversion 1.
 Qed.
 
 (* The only stuck term is [Fail]. *)
 
-Lemma only_fail_is_stuck {A} (m : free A) :
-  stuck m →
+Lemma only_fail_is_stuck {A} σ (m : free A) :
+  stuck (σ, m) →
   m = Fail.
 Proof.
   intros.
@@ -385,9 +467,9 @@ Qed.
 
 (* If [m] is stuck then [bind m f] is also stuck. *)
 
-Lemma stuck_bind {A B} (m : free A) (f : A → free B) :
-  stuck m →
-  stuck (bind m f).
+Lemma stuck_bind {A B} σ (m : free A) (f : A → free B) :
+  stuck (σ, m) →
+  stuck (σ, bind m f).
 Proof.
   intros.
   assert (m = Fail) by eauto using only_fail_is_stuck.
@@ -402,13 +484,13 @@ Qed.
 (* This principle allows case analyses with three cases, as follows:
    either [m] is a result, or [m] can step, or [m] is stuck. *)
 
-Lemma triplicity {A} (m : free A) :
+Lemma triplicity {A} σ (m : free A) :
   is_answer m ∨
-  can_step m ∨
-  stuck m.
+  can_step (σ, m) ∨
+  stuck (σ, m).
 Proof.
   destruct m; eauto using stuck_Fail with step is_answer.
 Qed.
 
-Ltac triplicity m H :=
-  destruct (triplicity m) as [ H | [ H | H ]].
+Ltac triplicity σ m H :=
+  destruct (triplicity σ m) as [ H | [ H | H ]].
