theories/store.v
@@ -1,0 +1,112 @@
+From stdpp Require Import countable numbers gmap.
+From iris.prelude Require Export prelude.
+From iris.prelude Require Import options.
+
+Require Import lang.
+
+
+(* TODO:
+ * - add the required lemmas so that the above types can remain opaque to the
+ *   rest of the development.
+ * - declare the required instances of [ElemOf] and [Dom].
+ *)
+
+(* -------------------------------------------------------------------------- *)
+(* Locations: The following section comes from the file 
+ * [iris_heap_lang/locations.v] available in the [iris] repository. *)
+
+Section Locations.
+
+  Record loc := Loc { loc_car : Z }.
+
+  Add Printing Constructor loc.
+
+  Global Instance loc_eq_decision : EqDecision loc.
+  Proof. solve_decision. Defined.
+
+  Global Instance loc_inhabited : Inhabited loc := populate {|loc_car := 0 |}.
+
+  Global Instance loc_countable : Countable loc.
+  Proof. by apply (inj_countable' loc_car Loc); intros []. Defined.
+
+  Global Program Instance loc_infinite : Infinite loc :=
+    inj_infinite (λ p, {| loc_car := p |}) (λ l, Some (loc_car l)) _.
+  Next Obligation. done. Qed.
+
+  Definition loc_add (l : loc) (off : Z) : loc :=
+    {| loc_car := loc_car l + off|}.
+
+  Notation "l +ₗ off" :=
+    (loc_add l off) (at level 50, left associativity) : stdpp_scope.
+
+  Lemma loc_add_assoc l i j : l +ₗ i +ₗ j = l +ₗ (i + j).
+  Proof. destruct l; rewrite /loc_add /=; f_equal; lia. Qed.
+
+  Lemma loc_add_0 l : l +ₗ 0 = l.
+  Proof. destruct l; rewrite /loc_add /=; f_equal; lia. Qed.
+
+  Global Instance loc_add_inj l : Inj eq eq (loc_add l).
+  Proof. destruct l; rewrite /Inj /loc_add /=; intros; simplify_eq; lia. Qed.
+
+  Definition fresh_locs (ls : gset loc) : loc :=
+    {| loc_car := set_fold (λ k r, (1 + loc_car k) `max` r)%Z 1%Z ls |}.
+
+  Lemma fresh_locs_fresh ls i :
+    (0 ≤ i)%Z → fresh_locs ls +ₗ i ∉ ls.
+  Proof.
+    intros Hi. cut (∀ l, l ∈ ls → loc_car l < loc_car (fresh_locs ls) + i)%Z.
+    { intros help Hf%help. simpl in *. lia. }
+    apply (set_fold_ind_L (λ r ls, ∀ l, l ∈ ls → (loc_car l < r + i)%Z));
+    set_solver by eauto with lia.
+  Qed.
+End Locations.
+
+(* -------------------------------------------------------------------------- *)
+(* The following section defines the physical store *)
+
+Section Store.
+  Definition store : Type := gmap loc val.
+
+
+  (* [store_ref] finds a fresh location to add to its argument.
+   * It returns the fresh location and the updated store. *)
+  Definition store_ref (s: store) (v: val) : loc * store :=
+    let l := fresh_locs (dom s) in
+    (l, <[l := v]>s).
+
+  Lemma store_ref_dom (s: store) (v: val) :
+    let '(l, s') := store_ref s v in
+    dom s' = (dom s) ∪ {[ l ]} ∧ l ∉ dom s.
+  Proof.
+    split; first set_solver.
+    unshelve epose proof (fresh_locs_fresh (dom s) 0 _) as H; first reflexivity.
+    rewrite loc_add_0 in H.
+    assumption.
+  Qed.
+
+
+  Global Instance val_inhabited: Inhabited val := populate VUnit.
+
+  (* [store_load] lookups the store to find a value given a location (which is 
+   * guaranteed to be valid). *)
+  (* TODO: directly write a term that represents this function. *)
+  Definition store_load (s: store) (l: loc) (Hsl: l ∈ dom s) : val.
+  Proof.
+    destruct (s !! l) eqn:E.
+    - exact v.
+    - apply lookup_lookup_total_dom in Hsl.
+      rewrite E in Hsl.
+      inversion Hsl.
+  Qed.
+
+
+  (* [store_store] updates a value of a store. The location that gets updated 
+   * has to be valid beforehand. This is enforced by the request of an argument 
+   * of type [l ∈ dom s]. *)
+  Definition store_store (s: store) (l: loc) (v: val) (_: l ∈ dom s) : store :=
+    <[ l := v ]> s.
+
+End Store.
+
+(*Global Opaque fresh_locs.
+Global Opaque store.*)
