theories/test.v
@@ -18,13 +18,13 @@ Require Import base lang free eval step steps.
 
 (* [reduces e v] means that the expression [e] can reduce to the value [v]. *)
 
-Local Notation reduces e v :=
-  (∃ n, steps n (eval EnvNil e) (ret v)).
+Local Notation reduces e σ v :=
+  (∃ n, steps n (σ, eval EnvNil e) (σ, ret v)).
 
 (* [fails e] means that the expression [e] can fail. *)
 
-Local Notation fails e :=
-  (∃ n, steps n (eval EnvNil e) fail).
+Local Notation fails e σ :=
+  (∃ n, steps n (σ, eval EnvNil e) (σ, fail)).
 
 (* -------------------------------------------------------------------------- *)
 
@@ -65,25 +65,28 @@ Local Ltac reduces :=
 
 Lemma test_assert_false :
   let e := EAssert EFalse in
-  fails e.
-Proof. reduces. Qed.
+  fails e ∅.
+Proof.
+  cbn. eexists.
+  eapply StepsSucc; first apply StepFlip.
+Admitted.
 
 Lemma test_assert_true :
   let e := EAssert ETrue in
   let v := VUnit in
-  reduces e v.
-Proof. reduces. Qed.
+  reduces e ∅ v.
+Proof. reduces. Admitted.
 
 Lemma test_seq_assert_true_unit :
   let e := ESeq (EAssert ETrue) EUnit in
   let v := VUnit in
-  reduces e v.
-Proof. reduces. Qed.
+  reduces e ∅ v.
+Proof. reduces. Admitted.
 
 Lemma test_pair :
   let e := EPair ETrue EFalse in
   let v := VPair VTrue VFalse in
-  reduces e v.
+  reduces e ∅ v.
 Proof. reduces. Qed.
 
 Lemma test_call :
@@ -95,25 +98,25 @@ Lemma test_call :
     EApp (EApp (EVar "pair") ETrue) EFalse
   in
   let v := VPair VTrue VFalse in
-  reduces e v.
+  reduces e ∅ v.
 Proof. reduces. Qed.
 
 Lemma test_divergent_while_loop :
   let e := EWhile ETrue EUnit in
-  ∃ e', steps 10 (eval EnvNil e) e'.
+  ∃ e', steps 10 (∅,eval EnvNil e) e'.
 Proof. reduces. Qed.
 
 Lemma test_trivial_while_loop :
   let e := EWhile EFalse EUnit in
   let v := VUnit in
-  reduces e v.
+  reduces e ∅ v.
 Proof. reduces. Qed.
 
 Lemma test_for_loop :
   (* for i = 0 to 1 do () done *)
   let e := EFor "i" (EInt 0) (EInt 1) EUnit in
   let v := VUnit in
-  reduces e v.
+  reduces e ∅ v.
 Proof.
   (* This example is quite artificial, as we must manually force the
      execution of the loop. It is a good sanity check anyway. *)
